chore: fix WF predicates

src/Std/Data/DHashMap/Basic.lean
@@ -333,11 +333,9 @@ section Unverified
   m.1.valuesArray
 
 /-- Computes the union of the given hash maps, inserting smaller list into a bigger list. In the case of clashes of keys, entries from the left argument, are replaced with entries from the right argument. -/
-@[inline] def union [BEq α] [Hashable α] (m₁ m₂ : DHashMap α β) : DHashMap α β := by
-  refine ⟨Raw₀.union ⟨m₁.1, m₁.2.size_buckets_pos⟩ ⟨m₂.1, m₂.2.size_buckets_pos⟩, ?_ ⟩
-  have := @Raw.WF.union α β _ _ m₁.1 m₂.1 m₁.2 m₂.2
-  simp [Std.DHashMap.Raw.union, m₁.2.size_buckets_pos, m₂.2.size_buckets_pos] at this
-  exact this
+@[inline] def union [BEq α] [Hashable α] (m₁ m₂ : DHashMap α β) : DHashMap α β where
+  inner := Raw₀.union ⟨m₁.1, m₁.2.size_buckets_pos⟩ ⟨m₂.1, m₂.2.size_buckets_pos⟩
+  wf := Std.DHashMap.Raw.WF.union₀ m₁.2 m₂.2
 
 instance [BEq α] [Hashable α] : Union (DHashMap α β) := ⟨union⟩
 
