src/Std/Data/DHashMap/Raw.lean
@@ -9,6 +9,7 @@ prelude
 public import Init.Data.BEq
 public import Init.Data.Hashable
 public import Std.Data.DHashMap.Internal.Defs
+import all Std.Data.DHashMap.Internal.Defs
 
 public section
 
@@ -705,10 +706,15 @@ theorem WF.Const.unitOfList [BEq α] [Hashable α] {l : List α} :
     (Const.unitOfList l : Raw α (fun _ => Unit)).WF :=
   Const.insertManyIfNewUnit WF.empty
 
+theorem WF.union₀ [BEq α] [Hashable α] {m₁ m₂ : Raw α β} (h₁ : m₁.WF) (h₂ : m₂.WF) : (Raw₀.union ⟨m₁, h₁.size_buckets_pos⟩ ⟨m₂, h₂.size_buckets_pos⟩).val.WF := by
+  simp only [Raw₀.union]
+  split
+  . exact (Raw₀.insertManyIfNew ⟨m₂, h₂.size_buckets_pos⟩ m₁).2 _ WF.insertIfNew₀ h₂
+  . exact (Raw₀.insertMany ⟨m₁, h₁.size_buckets_pos⟩ m₂).2 _ WF.insert₀ h₁
+
 theorem WF.union [BEq α] [Hashable α] {m₁ m₂ : Raw α β} (h₁ : m₁.WF) (h₂ : m₂.WF) : (m₁.union m₂ : Raw α β).WF := by
   simp [Std.DHashMap.Raw.union, h₁.size_buckets_pos, h₂.size_buckets_pos]
-  sorry
-
+  exact WF.union₀ h₁ h₂
 end WF
 
 end Raw
